coqimp/framework/logic/logic.v
@@ -1,4 +1,4 @@
-Require Import Coqlib.  
+Require Import Coqlib.   
 Require Import Maps. 
 
 Require Import Integers.
@@ -379,19 +379,19 @@ Inductive wf_seq : funspec -> asrt -> InsSeq -> asrt -> Prop :=
     (r2 |=> f2 ** p2) ==> fp L ** r -> fq L ** r ==> q -> DlyFrameFree r ->
     wf_seq Spec p (consJ2 f1 aexp1 r1 f2 aexp2 r2) q
 
-| Be_rule : forall p p' q r aexp f1 f2 f bv fp fq L i I Spec,
-    (p ↓) ==> (aexp ==ₓ f) -> Spec (f, f +ᵢ ($ 4)) = Some (fp, fq) ->
+| Be_rule : forall p p' q r f1 f2 f bv fp fq L i I Spec,
+    Spec (f, f +ᵢ ($ 4)) = Some (fp, fq) ->
     |- {{ p ↓↓ }} i {{ p' }} -> (p ↓) ==> z |=> bv ** Atrue ->
     wf_seq Spec ( p' //\\ [| bv =ᵢ ($ 0) = true |] ) I q -> DlyFrameFree r ->
     ((bv =ᵢ ($ 0) = false) -> ((p' ==> fp L ** r) /\ (fq L ** r ==> q))) ->
-    wf_seq Spec p (f1 e> be aexp ;; f2 e> i ;; I) q
+    wf_seq Spec p (f1 e> be f ;; f2 e> i ;; I) q
 
-| Bne_rule : forall p p' q r aexp f1 f2 f bv fp fq L i I Spec,
-    (p ↓) ==> (aexp ==ₓ f) -> Spec (f, f +ᵢ ($ 4)) = Some (fp, fq) ->
+| Bne_rule : forall p p' q r f1 f2 f bv fp fq L i I Spec,
+    Spec (f, f +ᵢ ($ 4)) = Some (fp, fq) ->
     |- {{ p ↓↓ }} i {{ p' }} -> (p ↓) ==> z |=> bv ** Atrue ->
     wf_seq Spec ( p' //\\ [| bv =ᵢ ($ 0) = false |] ) I q -> DlyFrameFree r ->
     ((bv =ᵢ ($ 0) = true) -> ((p' ==> fp L ** r) /\ (fq L ** r ==> q))) ->
-    wf_seq Spec p (f1 n> bne aexp ;; f2 n> i ;; I) q
+    wf_seq Spec p (f1 n> bne f ;; f2 n> i ;; I) q
 
 | Seq_frame_rule : forall p q I Spec r,
     wf_seq Spec p I q -> DlyFrameFree r ->
